Add the remaining `Array` theorems
This commit also fixes a bug in the backtracking behavior inside the
separation logic and Hoare logic tactics. The addition of the `ReaderT`
monad transformer in the past had changed the `MonadExcept` instance
used by the `try-catch` statement to no longer perform state restoration
on a failure as is done by `TacticM`. This commit re-enables that
behavior.

Co-authored-by: Marcin Kostrzewa <marckostrzewa@gmail.com>

stdlib/lampe/Stdlib/List.lean
@@ -22,13 +22,125 @@ def compareWith {α : Type}
 theorem compareWith_take_then_drop {α : Type} {a b : List α}
     (i : ℕ)
     (f : α → α → Ordering)
-  : compareWith f a b = 
+  : compareWith f a b =
     (compareWith f (a.take i) (b.take i)).then (compareWith f (a.drop i) (b.drop i)) := by
   induction i generalizing a b with
   | zero => simp_all
-  | succ n ih => 
+  | succ n ih =>
     cases a
     all_goals cases b
     any_goals rfl
     · simp [←ih, Ordering.then_assoc]
+
+/--
+States that the provided list is pairwise ordered according to the relation `f`.
+
+This is a strictly weaker notion than `List.Pairwise` or `List.Sorted` as it makes no claim as to
+the transitivity of the provided relation `f`, while those statements do so.
+
+This definition matches the notion of ordering used in `std::array::sort_via`, which does not (and
+cannot) check for global ordering by the relation `f`.
+-/
+def OrderedBy (f : α → α → Prop) (l : List α) : Prop :=
+  ∀i, (h : i < l.length - 1) → f l[i] l[i + 1]
+
+namespace OrderedBy
+
+theorem nil {f : α → α → Prop} : OrderedBy f [] := by simp_all [OrderedBy]
+
+theorem singleton {f : α → α → Prop} : OrderedBy f [x] := by simp_all [OrderedBy]
+
+theorem cons {f : α → α → Prop}
+  : f x y → OrderedBy f (y :: xs) → OrderedBy f (x :: y :: xs) := by
+  intro hh ht i hi
+
+  induction xs with
+  | nil =>
+    simp only [List.length_cons, List.length_nil, zero_add, Nat.reduceAdd, Nat.add_one_sub_one,
+      Nat.lt_one_iff] at hi
+    simp [hh, hi]
+  | cons z zs ih =>
+    simp at hi
+    cases i
+    · simp [hh]
+    · conv =>
+        congr
+        · rw [List.getElem_cons_succ]
+        · rw [List.getElem_cons_succ]
+      apply ht
+      simp_all
+
+theorem tail_cons {f : α → α → Prop} : OrderedBy f (x :: y :: xs) → OrderedBy f (y :: xs) := by
+  intro ha i hi
+  have := ha (i + 1) (by simp_all)
+  simp only [List.getElem_cons_succ] at this
+  assumption
+
+theorem cons_iff {f : α → α → Prop}
+  : f x y ∧ OrderedBy f (y :: xs) ↔ OrderedBy f (x :: y :: xs) := by
+  apply Iff.intro
+  · intro a
+    apply And.elim List.OrderedBy.cons a
+  · intro a
+    apply And.intro
+    · have := a 0
+      simp only [List.length_cons, add_tsub_cancel_right, lt_add_iff_pos_left, add_pos_iff,
+        zero_lt_one, or_true, List.getElem_cons_zero, zero_add, List.getElem_cons_succ,
+        forall_const] at this
+      assumption
+    · apply List.OrderedBy.tail_cons a
+
+theorem pair {f : α → α → Prop} : f x y ↔ List.OrderedBy f [x, y] := by
+  apply Iff.intro <;>
+  · intro hf
+    unfold OrderedBy at *
+    simp_all
+
+theorem trans_eq_Sorted {xs : List α} {f : α → α → Prop}
+  : OrderedBy f xs → Transitive f → List.Sorted f xs := by
+  intros ord trans
+
+  induction xs with
+  | nil => simp
+  | cons z zs ih =>
+    simp [List.Sorted.cons]
+
+    apply And.intro
+    · cases zs with
+      | nil => simp
+      | cons y ys =>
+        have := List.OrderedBy.cons_iff.mpr ord
+        have fzy := this.left
+        have tord := this.right
+        have rest_sorted := ih tord
+        have : IsTrans α f := ⟨trans⟩
+        have : List.Sorted f (z :: y :: ys) := List.sorted_cons_cons.mpr ⟨fzy, rest_sorted⟩
+        exact List.rel_of_sorted_cons this
+    · cases zs with
+      | nil => simp
+      | cons y ys => exact ih (List.OrderedBy.tail_cons ord)
+
+theorem append {α} {xs : List α} {h} {x} {f : α → α → Prop}
+  : (hf : f (xs.getLast h) x)
+  → (ord_pfx : OrderedBy f xs)
+  → OrderedBy f (xs ++ [x]) := by
+  intros hf ord_pfd
+
+  induction xs with
+  | nil => exact singleton
+  | cons y ys ih =>
+    cases ys with
+    | nil =>
+      simp_all only [ne_eq, not_true_eq_false, List.nil_append, IsEmpty.forall_iff,
+        List.getLast_singleton, List.cons_append]
+      exact pair.mp hf
+    | cons z zs =>
+      have hne : z :: zs ≠ [] := by simp_all
+      have ho : OrderedBy f (z :: zs) := (cons_iff.mpr ord_pfd).right
+      have hf : f ((z :: zs).getLast (by omega)) x := by simp_all
+      have ih := @ih (by assumption) (by assumption) (by assumption)
+      simp only [List.cons_append] at *
+      apply cons ((cons_iff.mpr ord_pfd).left) ih
+
+end OrderedBy
 
