Lampe/Lampe/Tactic/Steps.lean
@@ -139,6 +139,9 @@ def getClosingTerm (val : Lean.Expr) : TacticM (Option (TSyntax `term)) := withT
         | ``Lampe.Builtin.strAsBytes => return some (←``(strAsBytes_intro))
         | ``Lampe.Builtin.arrayAsStrUnchecked => return some (←``(arrayAsStrUnchecked_intro))
 
+        | ``Lampe.Builtin.isUnconstrained => 
+          return some (←``(genericTotalPureBuiltin_intro Builtin.isUnconstrained rfl))
+
         -- Array builtins
         | ``Lampe.Builtin.mkArray =>
           let some argTypes := val.getAppArgs[1]? | throwError "malformed mkSlice"
