stdlib/lampe/Stdlib/Array/Mod.lean
@@ -1,9 +1,499 @@
 import «std-1.0.0-beta.12».Extracted
+import Stdlib.Array.CheckShuffle
+import Stdlib.Convert
+import Stdlib.Tp
+
+import Batteries.Classes.Order
 import Lampe
 
 namespace Lampe.Stdlib.Array
+namespace Lampe.Stdlib.List
 
 open «std-1.0.0-beta.12»
+
+set_option Lampe.pp.Expr true
+set_option Lampe.pp.STHoare true
+
+theorem map_spec {p T N U Env l f fb}
+    (inv : List (T.denote p) → List (U.denote p) → SLP (State p))
+    (inv_spec : ∀(ip : List (T.denote p)) (op : List (U.denote p)) (e : T.denote p),
+      (ip ++ [e] <+: l.toList) → STHoare p env (inv ip op) (fb h![e])
+        (fun r => inv (ip ++ [e]) (op ++ [r])))
+  : STHoare p env
+    ((inv [] []) ⋆ [λf ↦ fb])
+    («std-1.0.0-beta.12::array::map».call h![T, N, U, Env] h![l, f])
+    (fun r => inv l.toList r.toList ⋆ [λf ↦ fb]) := by
+  enter_decl
+  steps
+  loop_inv nat fun i _ _ => ∃∃v,
+    [ret ↦ ⟨U.array N, v⟩] ⋆ (inv (l.take i).toList (v.take i).toList) ⋆ [λf ↦ fb]
+  · sl
+  · simp
+  · intro i hlo hhi
+    steps
+    simp_all only [BitVec.toNat_intCast, Int.reducePow, EuclideanDomain.zero_mod, Int.toNat_zero,
+      zero_le, List.Vector.toList_take, Builtin.instCastTpU, BitVec.truncate_eq_setWidth,
+      BitVec.setWidth_eq, BitVec.toNat_ofNatLT]
+    generalize_proofs
+    rename_i i_lt_pow
+
+    rename Tp.denote p (U.array N) => v
+    have := inv_spec (l.take i).toList (v.take i).toList (l.toList[i]'(by simp_all))
+      (by simp [List.take_prefix])
+    steps [STHoare.callLambda_intro (hlam := this)]
+    simp_all only [Builtin.instCastTpU, BitVec.truncate_eq_setWidth, BitVec.setWidth_eq,
+      BitVec.toNat_ofNatLT, List.Vector.toList_take, List.take_append_getElem, Lens.modify,
+      Lens.get, Access.modify, ↓reduceDIte, Option.bind_eq_bind, Option.bind_some,
+      Option.bind_fun_some, Option.get_some, List.Vector.toList_set]
+
+    have : i < (v.toList.set i «#v_5»).length := by simp_all
+    conv => rhs; enter [1, 2]; rw [List.take_succ_eq_append_getElem this]
+    simp only [List.getElem_set this, if_true]
+    conv =>
+      rhs
+      enter [1, 2, 1]
+      apply List.take_set_of_le (by rfl)
+
+    sl
+
+  steps
+  simp_all only [BitVec.toNat_intCast, Int.reducePow, EuclideanDomain.zero_mod, Int.toNat_zero,
+    BitVec.natCast_eq_ofNat, BitVec.ofNat_toNat, BitVec.setWidth_eq, zero_le,
+    List.Vector.toList_take]
+
+  rename Tp.denote p (U.array N) => v
+  rename_i a
+  have l1 : BitVec.toNat N = l.toList.length := by simp
+  have l2 : BitVec.toNat N = v.toList.length := by simp
+
+  conv =>
+    lhs
+    rhs
+    congr
+    · arg 1; apply l1
+    · arg 1; apply l2
+
+  simp only [a, List.take_length]
+  sl
+
+theorem map_pure_spec {p T N U Env l f fb fEmb}
+    (inv_pure : ∀a, STHoare p env ⟦⟧ (fb h![a]) (fun r => r = fEmb a))
+  : STHoare p env [λf ↦ fb]
+    («std-1.0.0-beta.12::array::map».call h![T, N, U, Env] h![l, f])
+    (fun r => r.toList = l.toList.map fEmb) := by
+  steps [map_spec (inv := fun i o => o = i.map fEmb)]
+  · simp
+  · assumption
+  · intros; steps [inv_pure]; simp_all
+
+theorem mapi_spec {p T N U Env l f fb}
+    (inv : List (T.denote p) → List (U.denote p) → SLP (State p))
+    (inv_spec : ∀(ip : List (T.denote p)) (op : List (U.denote p)) (e : T.denote p),
+      ((ip ++ [e]) <+: l.toList) → STHoare p env (inv ip op) (fb h![ip.length, e])
+        (fun r => inv (ip ++ [e]) (op ++ [r])))
+  : STHoare p env
+    (inv [] [] ⋆ [λf ↦ fb])
+    («std-1.0.0-beta.12::array::mapi».call h![T, N, U, Env] h![l, f])
+    (fun r => inv l.toList r.toList ⋆ [λf ↦ fb]) := by
+  enter_decl
+  steps
+  loop_inv nat fun i _ _ =>
+    ∃∃v, [ret ↦ ⟨U.array N, v⟩] ⋆ inv (l.take i).toList (v.take i).toList ⋆ [λf ↦ fb]
+  · sl
+  · simp
+  · intro i hlo hhi
+    steps
+    simp_all only [BitVec.natCast_eq_ofNat, BitVec.toNat_intCast, Int.reducePow,
+      EuclideanDomain.zero_mod, Int.toNat_zero, zero_le, List.Vector.toList_take,
+      Builtin.instCastTpU, BitVec.truncate_eq_setWidth, BitVec.setWidth_eq, BitVec.toNat_ofNatLT]
+    generalize_proofs
+    rename_i i_lt_pow i_lt_n
+
+    rename Tp.denote p (U.array N) => v
+    have := inv_spec (l.take i).toList (v.take i).toList (l.toList[i]'(by simp_all))
+      (by simp [List.take_prefix])
+    have i_eq_len_take : BitVec.ofNatLT i i_lt_pow = BitVec.ofNat 32 (l.take i).toList.length := by
+      simp_all only [Builtin.instCastTpU, BitVec.truncate_eq_setWidth, BitVec.setWidth_eq,
+        BitVec.toNat_ofNatLT, Nat.reducePow, List.Vector.toList_take, List.length_take,
+        List.Vector.toList_length, List.take_append_getElem, BitVec.natCast_eq_ofNat]
+      congr
+      omega
+    simp only [i_eq_len_take]
+
+    steps [STHoare.callLambda_intro (hlam := this)]
+    simp_all only [Builtin.instCastTpU, BitVec.truncate_eq_setWidth, BitVec.setWidth_eq,
+      List.Vector.toList_take, List.length_take, List.Vector.toList_length, BitVec.toNat_ofNat,
+      Nat.reducePow, List.take_append_getElem, Lens.modify, Lens.get, Access.modify, ↓reduceDIte,
+      Option.bind_eq_bind, Option.bind_some, Option.bind_fun_some, Option.get_some,
+      List.Vector.toList_set]
+
+    have : (min i N.toNat) % 4294967296 = i := by omega
+    rw [this]
+    have : i < (v.toList.set i «#v_5»).length := by simp_all
+    conv => rhs; enter [1, 2]; rw [List.take_succ_eq_append_getElem this]
+    simp only [List.getElem_set this, if_true]
+    conv => rhs; enter [1, 2, 1]; apply List.take_set_of_le (by rfl)
+    sl
+
+  steps
+  simp_all only [BitVec.natCast_eq_ofNat, BitVec.toNat_intCast, Int.reducePow,
+    EuclideanDomain.zero_mod, Int.toNat_zero, BitVec.ofNat_toNat, BitVec.setWidth_eq, zero_le,
+    List.Vector.toList_take]
+
+  rename Tp.denote p (U.array N) => v
+  rename_i a
+  have l1 : BitVec.toNat N = l.toList.length := by simp
+  have l2 : BitVec.toNat N = v.toList.length := by simp
+  conv =>
+    lhs
+    rhs
+    congr
+    · arg 1; apply l1
+    · arg 1; apply l2
+
+  simp only [a, List.take_length]
+  sl
+
+theorem mapi_pure_spec {p T N U Env l f fb fEmb}
+    (inv_pure : ∀i x, (h : i < l.length) → STHoare p env ⟦⟧ (fb h![i, x]) (fun r => r = fEmb i x))
+  : STHoare p env [λf ↦ fb]
+    («std-1.0.0-beta.12::array::mapi».call h![T, N, U, Env] h![l, f])
+    (fun r => r.toList = l.toList.mapIdx fEmb) := by
+  steps [mapi_spec (inv := fun i o => o = i.mapIdx fEmb)]
+  · simp
+  · assumption
+  · intros;
+    rename List (T.denote p) => ip
+    rename T.denote p => e
+    steps [inv_pure ip.length e ?lt]
+    case lt =>
+      rename_i a
+      simp_all only [BitVec.natCast_eq_ofNat]
+      have h1 : (ip ++ [e]).length ≤ l.toList.length := List.IsPrefix.length_le a
+      have h2 : l.toList.length = l.length := by simp
+      rw [h2, List.length_append] at h1
+      exact h1
+
+    simp_all
+
+theorem for_each_spec {p T N Env l f fb}
+    (inv : List (T.denote p) → SLP (State p))
+    (inv_spec : ∀(ip : List (T.denote p)) (e : T.denote p),
+      ((ip ++ [e]) <+: l.toList) → STHoare p env (inv ip) (fb h![e]) (fun _ => inv (ip ++ [e])))
+  : STHoare p env
+    (inv [] ⋆ [λf ↦ fb])
+    («std-1.0.0-beta.12::array::for_each».call h![T, N, Env] h![l, f])
+    (fun _ => inv l.toList ⋆ [λf ↦ fb]) := by
+  enter_decl
+  steps
+  loop_inv nat fun i _ _ => inv (l.take i).toList ⋆ [λf ↦ fb]
+  · simp
+  · intro i hlo hhi
+    steps
+    simp_all only [BitVec.toNat_intCast, Int.reducePow, EuclideanDomain.zero_mod, Int.toNat_zero,
+      zero_le, List.Vector.toList_take, Builtin.instCastTpU, BitVec.truncate_eq_setWidth,
+      BitVec.setWidth_eq, BitVec.toNat_ofNatLT]
+    generalize_proofs
+
+    have := inv_spec (l.take i).toList (l.toList[i]'(by simp_all)) (by simp [List.take_prefix])
+    steps [STHoare.callLambda_intro (hlam := this)]
+    simp_all only [Builtin.instCastTpU, BitVec.truncate_eq_setWidth, BitVec.setWidth_eq,
+      BitVec.toNat_ofNatLT, List.Vector.toList_take, List.take_append_getElem]
+    sl
+
+  steps
+  simp_all only [BitVec.toNat_intCast, Int.reducePow, EuclideanDomain.zero_mod, Int.toNat_zero,
+    BitVec.natCast_eq_ofNat, BitVec.ofNat_toNat, BitVec.setWidth_eq, zero_le,
+    List.Vector.toList_take]
+  have l1 : BitVec.toNat N = l.toList.length := by simp
+  conv => lhs; enter [1, 1]; rw [l1]
+  simp only [List.take_length]
+  sl
+
+theorem for_eachi_spec {p T N Env l f fb}
+    (inv : List (T.denote p) → SLP (State p))
+    (inv_spec : ∀(ip : List (T.denote p)) (e : T.denote p),
+      ((ip ++ [e] <+: l.toList) → STHoare p env (inv ip) (fb h![ip.length, e]) (fun _ => inv (ip ++ [e]))))
+  : STHoare p env
+    (inv [] ⋆ [λf ↦ fb])
+    («std-1.0.0-beta.12::array::for_eachi».call h![T, N, Env] h![l, f])
+    (fun _ => inv l.toList ⋆ [λf ↦ fb]) := by
+  enter_decl
+  steps
+  loop_inv nat fun i _ _ => inv (l.take i).toList ⋆ [λf ↦ fb]
+  · simp
+  · intro i hlo hhi
+    steps
+    simp_all only [BitVec.natCast_eq_ofNat, BitVec.toNat_intCast, Int.reducePow,
+      EuclideanDomain.zero_mod, Int.toNat_zero, zero_le, List.Vector.toList_take,
+      Builtin.instCastTpU, BitVec.truncate_eq_setWidth, BitVec.setWidth_eq, BitVec.toNat_ofNatLT]
+    generalize_proofs
+    rename_i i_lt_pow i_lt_n
+
+    have := inv_spec (l.take i).toList (l.toList[i]'(by simp_all)) (by simp [List.take_prefix])
+    have i_eq_len_take : BitVec.ofNatLT i i_lt_pow = BitVec.ofNat 32 (l.take i).toList.length := by
+      simp_all only [Builtin.instCastTpU, BitVec.truncate_eq_setWidth, BitVec.setWidth_eq,
+        BitVec.toNat_ofNatLT, Nat.reducePow, List.Vector.toList_take, List.length_take,
+        List.Vector.toList_length, List.take_append_getElem, BitVec.natCast_eq_ofNat]
+      congr
+      omega
+    simp only [i_eq_len_take]
+    steps [STHoare.callLambda_intro (hlam := this)]
+
+    simp_all only [Builtin.instCastTpU, BitVec.truncate_eq_setWidth, BitVec.setWidth_eq,
+      List.Vector.toList_take, List.length_take, List.Vector.toList_length, BitVec.toNat_ofNat,
+      Nat.reducePow, List.take_append_getElem]
+    sl
+
+  steps
+  simp_all only [BitVec.natCast_eq_ofNat, BitVec.toNat_intCast, Int.reducePow,
+    EuclideanDomain.zero_mod, Int.toNat_zero, BitVec.ofNat_toNat, BitVec.setWidth_eq, zero_le,
+    List.Vector.toList_take]
+  have l1 : BitVec.toNat N = l.toList.length := by simp
+  conv => lhs; enter [1, 1]; rw [l1]
+  simp only [List.take_length]
+  sl
+
+theorem fold_spec {p T N U Env l a f fb}
+    (inv : List (T.denote p) → U.denote p → SLP (State p))
+    (inv_spec : ∀(ip : List (T.denote p)) (accum : U.denote p) (e : T.denote p),
+      ((ip ++ [e] <+: l.toList) → STHoare p env (inv ip accum) (fb h![accum, e])
+        (fun r => inv (ip ++ [e]) r)))
+  : STHoare p env
+    (inv [] a ⋆ [λf ↦ fb])
+    («std-1.0.0-beta.12::array::fold».call h![T, N, U, Env] h![l, a, f])
+    (fun r => (inv l.toList r) ⋆ [λf ↦ fb]) := by
+  enter_decl
+  steps
+  step_as ([accumulator ↦ ⟨U, a⟩] ⋆ [λf ↦ fb] ⋆ inv [] a)
+    (fun _ => ∃∃v, [accumulator ↦ ⟨U, v⟩] ⋆ [λf ↦ fb] ⋆ inv l.toList v)
+  steps
+  loop_inv nat fun i _ _ => ∃∃v, [accumulator ↦ ⟨U, v⟩] ⋆ [λf ↦ fb] ⋆ inv (l.take i).toList v
+  · sl
+  · simp
+  · intro i hlo hhi
+    steps
+    simp_all only [BitVec.toNat_intCast, Int.reducePow, EuclideanDomain.zero_mod, Int.toNat_zero,
+      zero_le, Builtin.instCastTpU, BitVec.truncate_eq_setWidth, BitVec.setWidth_eq,
+      BitVec.toNat_ofNatLT, List.Vector.toList_take]
+    generalize_proofs
+    rename U.denote p => v
+
+    have := inv_spec (l.take i).toList v (l.toList[i]'(by simp_all)) (by simp [List.take_prefix])
+    steps [STHoare.callLambda_intro (hlam := this)]
+
+    simp_all only [List.Vector.toList_take, List.take_append_getElem, Lens.modify, Option.get_some]
+    sl
+
+  steps
+  simp_all only [BitVec.toNat_intCast, Int.reducePow, EuclideanDomain.zero_mod, Int.toNat_zero,
+    BitVec.natCast_eq_ofNat, BitVec.ofNat_toNat, BitVec.setWidth_eq, zero_le,
+    List.Vector.toList_take]
+
+  have l1 : BitVec.toNat N = l.toList.length := by simp
+  simp only [l1, List.take_length]
+  sl
+
+  steps
+  subst_vars
+  sl
+
+theorem fold_pure_spec {p T N U Env l a f fb fEmb}
+    (inv_pure : ∀a x, STHoare p env ⟦⟧ (fb h![a, x]) (fun r => r = fEmb a x))
+  : STHoare p env [λf ↦ fb]
+    («std-1.0.0-beta.12::array::fold».call h![T, N, U, Env] h![l, a, f])
+    (fun r => r = l.toList.foldl fEmb a ⋆ [λf ↦ fb]) := by
+  steps [fold_spec (inv := fun xs v => v = xs.foldl fEmb a)]
+  · rfl
+  · assumption
+  · intros; steps [inv_pure]; simp_all
+
+theorem reduce_spec {p T N Env l f fb}
+    (l_len_gt : l.length > 0)
+    (inv : List (T.denote p) → T.denote p → SLP (State p))
+    (inv_spec : ∀(ip : List (T.denote p)) (acc : T.denote p) (e : T.denote p),
+      ((ip ++ [e] <+: l.toList.tail) → STHoare p env (inv ip acc) (fb h![acc, e])
+        (fun r => inv (ip ++ [e]) r)))
+  : STHoare p env
+    (inv [] l[0] ⋆ [λf ↦ fb])
+    («std-1.0.0-beta.12::array::reduce».call h![T, N, Env] h![l, f])
+    (fun r => inv l.toList.tail r ⋆ [λf ↦ fb]) := by
+  enter_decl
+  steps
+  rcases l_def : l with ⟨ts, l_prf⟩
+  have ts_len_gt_0 : ts.length > 0 := by omega
+  cases ts with
+  | nil => contradiction
+  | cons init r =>
+    have r_len_succ_eq_n : r.length + 1 = N.toNat := l_prf
+    simp only [List.Vector.toList_mk, List.tail_cons, List.length_cons, gt_iff_lt,
+      lt_add_iff_pos_left, add_pos_iff, zero_lt_one, or_true, BitVec.toNat_intCast, Int.reducePow,
+      EuclideanDomain.zero_mod, Int.toNat_zero, BitVec.natCast_eq_ofNat, BitVec.ofNat_toNat,
+      BitVec.setWidth_eq] at *
+    loop_inv nat fun i _ _ => ∃∃v, [accumulator ↦ ⟨T, v⟩] ⋆ [λf ↦ fb] ⋆ inv (r.take (i - 1)) v
+    · sl
+    · simp only [BitVec.toNat_intCast, Int.reducePow, Int.reduceMod, Int.toNat_one]; omega
+    · intro i hlo hhi
+      cases i with
+      | zero => contradiction
+      | succ i =>
+        steps
+        simp_all only [BitVec.toNat_intCast, Int.reducePow, EuclideanDomain.zero_mod,
+          Int.toNat_zero, gt_iff_lt, Int.reduceMod, Int.toNat_one, le_add_iff_nonneg_left, zero_le,
+          add_tsub_cancel_right, Builtin.instCastTpU, BitVec.truncate_eq_setWidth,
+          BitVec.setWidth_eq, BitVec.toNat_ofNatLT]
+        generalize_proofs
+        rename T.denote p => v
+
+        have i_lt_r_length : i < r.length := by
+          have : (init :: r).length = N.toNat := by simp_all
+          have : i + 1 < N.toNat := by linarith
+          omega
+
+        have := inv_spec (r.take i) v r[i] (by simp [List.take_prefix])
+        have get_eq_getElem : List.Vector.get ⟨init :: r, l_prf⟩ ⟨i + 1, hhi⟩ = r[i] := by rfl
+        rw [get_eq_getElem]
+
+        steps [STHoare.callLambda_intro (hlam := this)]
+        simp_all only [Builtin.instCastTpU, BitVec.truncate_eq_setWidth, BitVec.setWidth_eq,
+          BitVec.toNat_ofNatLT, List.Vector.toList_mk, List.tail_cons, List.take_append_getElem,
+          Lens.modify, Option.get_some]
+        sl
+
+    steps
+    simp_all only [gt_iff_lt, List.Vector.toList_mk, List.tail_cons, BitVec.toNat_intCast,
+      Int.reducePow, EuclideanDomain.zero_mod, Int.toNat_zero, Int.reduceMod, Int.toNat_one]
+    have : r.length = N.toNat - 1 := by omega
+    rw [←this, List.take_length]
+    subst_vars
+    sl
+
+theorem reduce_pure_spec {p T N Env l f fb fEmb}
+    (l_len_gt : l.length > 0)
+    (inv_pure : ∀a x, STHoare p env ⟦⟧ (fb h![a, x]) (fun r => r = fEmb a x))
+  : STHoare p env [λf ↦ fb]
+    («std-1.0.0-beta.12::array::reduce».call h![T, N, Env] h![l, f])
+    (fun r => r = l.toList.tail.foldl fEmb l[0] ⋆ [λf ↦ fb]) := by
+  steps [reduce_spec (inv := fun xs v => v = xs.foldl fEmb l[0])]
+  · rfl
+  · assumption
+  · intros; steps [inv_pure]; simp_all
+
+theorem all_spec {p T N Env l f fb}
+    (inv : List (T.denote p) → Bool → SLP (State p))
+    (inv_spec : ∀(ip : List (T.denote p)) (op : Bool) (e : T.denote p),
+      ((ip ++ [e] <+: l.toList) → STHoare p env (inv ip op) (fb h![e])
+        (fun r => inv (ip ++ [e]) (op ∧ r))))
+  : STHoare p env
+    (inv [] true ⋆ [λf ↦ fb])
+    («std-1.0.0-beta.12::array::all».call h![T, N, Env] h![l, f])
+    (fun r => inv l.toList r ⋆ [λf ↦ fb]) := by
+  enter_decl
+  steps
+  step_as ([ret ↦ ⟨.bool, true⟩] ⋆ (inv [] true) ⋆ [λf ↦ fb])
+    (fun r => ∃∃b, [ret ↦ ⟨.bool, b⟩] ⋆ (inv l.toList b) ⋆ [λf ↦ fb])
+
+  steps
+  loop_inv nat fun i _ _ => ∃∃b, [ret ↦ ⟨.bool, b⟩] ⋆ (inv (l.toList.take i) b) ⋆ [λf ↦ fb]
+  · sl
+  · simp
+  · intro i hlo hhi
+    steps
+    simp_all only [BitVec.toNat_intCast, Int.reducePow, EuclideanDomain.zero_mod, Int.toNat_zero,
+      zero_le, Builtin.instCastTpU, BitVec.truncate_eq_setWidth, BitVec.setWidth_eq,
+      BitVec.toNat_ofNatLT]
+    generalize_proofs
+    rename Tp.denote p .bool => b
+
+    have := inv_spec (l.toList.take i) b (l.toList[i]'(by simp_all)) (by simp [List.take_prefix])
+    steps [STHoare.callLambda_intro (hlam := this)]
+    simp_all only [Bool.decide_and, Bool.decide_eq_true, Bool.forall_bool, Bool.false_and,
+      Bool.true_and, List.take_append_getElem, Lens.modify, Option.get_some]
+    sl
+    exact ()
+  · simp_all only [Bool.decide_and, Bool.decide_eq_true, Bool.forall_bool, Bool.false_and,
+    Bool.true_and, BitVec.natCast_eq_ofNat, BitVec.ofNat_toNat, BitVec.setWidth_eq, SLP.star_true]
+    steps
+
+    have : l.toList.length = N.toNat := by simp
+    simp only [←this, List.take_length]
+    sl
+
+  steps
+  subst_vars
+  sl
+
+theorem all_pure_spec {p T N Env l f fb fEmb}
+    (inv_pure : ∀a, STHoare p env ⟦⟧ (fb h![a]) (fun r => r = fEmb a))
+  : STHoare p env [λf ↦ fb]
+    («std-1.0.0-beta.12::array::all».call h![T, N, Env] h![l, f])
+    (fun r => r = l.toList.all fEmb) := by
+  steps [all_spec (inv := fun x r => r = x.all fEmb)]
+  · simp
+  · assumption
+  · intro ip op e pfx
+    steps [inv_pure]
+    simp_all only [List.all_eq_true, Bool.decide_and, Bool.decide_eq_true, List.all_append,
+      List.all_cons, List.all_nil, Bool.and_true]
+    rw [←List.all_eq]
+
+theorem any_spec {p T N Env l f fb}
+    (inv : List (T.denote p) → Bool → SLP (State p))
+    (inv_spec : ∀(ip : List (T.denote p)) (op : Bool) (e : T.denote p),
+      ((ip ++ [e] <+: l.toList) → STHoare p env (inv ip op) (fb h![e])
+        (fun r => inv (ip ++ [e]) (op ∨ r))))
+  : STHoare p env
+    (inv [] false ⋆ [λf ↦ fb])
+    («std-1.0.0-beta.12::array::any».call h![T, N, Env] h![l, f])
+    (fun r => inv l.toList r ⋆ [λf ↦ fb]) := by
+  enter_decl
+  steps
+  step_as ([ret ↦ ⟨.bool, false⟩] ⋆ (inv [] false) ⋆ [λf ↦ fb])
+    (fun r => ∃∃b, [ret ↦ ⟨.bool, b⟩] ⋆ (inv l.toList b) ⋆ [λf ↦ fb])
+
+  steps
+  loop_inv nat fun i _ _ => ∃∃b, [ret ↦ ⟨.bool, b⟩] ⋆ (inv (l.toList.take i) b) ⋆ [λf ↦ fb]
+  · sl
+  · simp
+  · intro i hlo hhi
+    steps
+    simp_all only [BitVec.toNat_intCast, Int.reducePow, EuclideanDomain.zero_mod, Int.toNat_zero,
+      zero_le, Builtin.instCastTpU, BitVec.truncate_eq_setWidth, BitVec.setWidth_eq,
+      BitVec.toNat_ofNatLT]
+    generalize_proofs
+    rename Tp.denote p .bool => b
+
+    have := inv_spec (l.toList.take i) b (l.toList[i]'(by simp_all)) (by simp [List.take_prefix])
+    steps [STHoare.callLambda_intro (hlam := this)]
+    simp_all only [Bool.decide_or, Bool.decide_eq_true, Bool.forall_bool, Bool.false_or,
+      Bool.true_or, List.take_append_getElem, Lens.modify, Option.get_some]
+    sl
+    exact ()
+  · simp_all only [Bool.decide_and, Bool.decide_eq_true, Bool.forall_bool, Bool.false_and,
+    Bool.true_and, BitVec.natCast_eq_ofNat, BitVec.ofNat_toNat, BitVec.setWidth_eq, SLP.star_true]
+    steps
+
+    have : l.toList.length = N.toNat := by simp
+    simp only [←this, List.take_length]
+    sl
+
+  steps
+  subst_vars
+  sl
+
+theorem any_pure_spec {p T N Env l f fb fEmb}
+    (inv_pure : ∀a, STHoare p env ⟦⟧ (fb h![a]) (fun r => r = fEmb a))
+  : STHoare p env [λf ↦ fb]
+    («std-1.0.0-beta.12::array::any».call h![T, N, Env] h![l, f])
+    (fun r => r = l.toList.any fEmb) := by
+  steps [any_spec (inv := fun x r => r = x.any fEmb)]
+  · simp
+  · assumption
+  · intro ip op e pfx
+    steps [inv_pure]
+    simp_all only [List.any_eq_true, Bool.decide_or, Bool.decide_eq_true, List.any_append,
+      List.any_cons, List.any_nil, Bool.or_false]
+    rw [←List.any_eq]
 
 theorem concat_spec: STHoare p env ⟦⟧
     («std-1.0.0-beta.12::array::concat».call h![T, M, N] h![a₁, a₂])
@@ -61,4 +551,231 @@ theorem concat_spec: STHoare p env ⟦⟧
   rw [List.take_of_length_le ?le1, List.take_of_length_le ?le2] at hp
   case le1 => simp [Nat.mod_le]
   case le2 => simp
+  simp_all
+
+/--
+This theorem asserts that `std::array::sort_via` implements a valid sort (namely that the output is
+a sorted permutation of the input) but does not make any requirements on _how_ the sort is done.
+
+It makes no guarantees as to the computational complexity or stability of the sort, but does ensure
+that the result is ordered by the provided relation and that its elements represent a valid
+permutation of the input.
+
+Do note that the function as written can only assume that the elements are pairwise ordered by the
+provided comparator function. In other words, it does **not** guarantee that they are sorted unless
+the comparator function is transitive. For a more strict version of this theorem, see
+`sort_via_trans_spec`, which uses a proof of transitivity for the comparator to assure that the
+output is sorted.
+
+Note that we have intentionally omitted an impure theorem for `sort_via` as we can envision no sane
+use-case for impure comparator functions.
+-/
+theorem sort_via_spec {p T N Env l f fb}
+    {t_eq : Cmp.Eq.hasImpl env T}
+    (t_eq_spec : ∀a b, STHoare p env ⟦⟧ (Cmp.Eq.eq h![] T h![] h![] h![a, b])
+      (fun r : Bool => ⟦r ↔ a = b⟧))
+    {fEmb : T.denote p → T.denote p → Bool}
+    (f_spec : ∀a b, STHoare p env ⟦⟧ (fb h![a, b]) (fun r => r = fEmb a b))
+  : STHoare p env [λf ↦ fb]
+    («std-1.0.0-beta.12::array::sort_via».call h![T, N, Env] h![l, f])
+    (fun r => List.OrderedBy (fEmb · · = true) r.toList ∧ List.Perm l.toList r.toList) := by
+  enter_decl
+
+  let r_def := fun a b => fEmb a b = true
+
+  -- The call to `std::array::quicksort::quicksort` is just an unconstrained function, so returns
+  -- a fresh value. We can say nothing else about it.
+  step_as ([λf ↦ fb]) (fun _ => [λf ↦ fb])
+  · steps
+    enter_decl
+    steps
+
+  steps
+  any_goals exact ()
+
+  step_as ([λf ↦ fb]) (fun _ => [λf ↦ fb] ⋆
+    List.OrderedBy r_def sorted.toList ∧ List.Perm l.toList sorted.toList)
+
+  apply STHoare.ite_intro
+  any_goals intros; contradiction
+
+  intro cond
+  steps
+
+  rename_i one_lt_n
+  have zero_lt_n : 0 < N.toNat := by
+    simp_all only [Bool.not_false, BitVec.ofNat_eq_ofNat]
+    exact one_lt_n
+  have n_eq_len : sorted.toList.length = N.toNat := by simp_all
+
+  loop_inv nat fun i _ _ => [λf ↦ fb] ⋆ List.OrderedBy r_def (sorted.toList.take (i + 1))
+  · simp only [BitVec.toNat_intCast, Int.reducePow, EuclideanDomain.zero_mod, Int.toNat_zero,
+      zero_add]
+
+    rw [List.take_add_one, List.take_zero, List.getElem?_eq_getElem (by omega)]
+    apply List.OrderedBy.singleton
+  · simp
+  · intro i hlo hhi
+    steps
+    rename List.OrderedBy _ _ => pfx_ordered
+
+    simp_all only [Bool.not_false, List.Vector.toList_length, BitVec.toNat_intCast, Int.reducePow,
+      EuclideanDomain.zero_mod, Int.toNat_zero, zero_le, BitVec.toNat_ofNatLT, Int.reduceMod,
+      Int.toNat_one, Nat.reducePow, Builtin.instCastTpU, BitVec.truncate_eq_setWidth,
+      BitVec.setWidth_eq, BitVec.toNat_add]
+
+    rename_i i_succ_lt_2pow
+    conv => enter [4, 1, 4, 2, 1, 2, 1]; rw [Nat.mod_eq_of_lt i_succ_lt_2pow]
+
+    generalize_proofs
+    rename_i i_lt_n i_succ_lt_n
+    generalize ith_def : sorted.get ⟨i, i_lt_n⟩ = ith at *
+    generalize isth_def : sorted.get ⟨i + 1, i_succ_lt_n⟩ = isth at *
+
+    have := f_spec ith isth
+    steps [STHoare.callLambda_intro (hlam := this)]
+    rw [List.take_succ_eq_append_getElem (by simp_all)]
+
+    have : sorted.toList ≠ [] := by
+      have : N.toNat ≠ 0 := by omega
+      have : N.toNat = sorted.toList.length := by simp_all
+      apply List.length_pos_iff_ne_nil.mp (by omega)
+
+    have : List.take (i + 1) (List.Vector.toList sorted) ≠ [] := by
+      rw [List.take_succ_eq_append_getElem (by simp_all)]
+      apply List.append_ne_nil_of_right_ne_nil
+      simp
+
+    apply List.OrderedBy.append (h := this) (ord_pfx := pfx_ordered)
+
+    generalize_proofs pf₁ pf₂
+    have : (sorted.toList.take (i + 1)).getLast this = sorted[i] := by
+      simp only [List.getLast_take, add_tsub_cancel_right]
+      rw [List.getElem?_eq_getElem (by simp_all), Option.getD_some]
+      apply List.Vector.toList_getElem
+    rw [this, List.Vector.toList_getElem]
+    unfold r_def
+    simp_all only [Builtin.instCastTpU, BitVec.truncate_eq_setWidth, BitVec.setWidth_eq,
+      BitVec.toNat_ofNatLT, BitVec.toNat_add, BitVec.toNat_intCast, Int.reducePow, Int.reduceMod,
+      Int.toNat_one, Nat.reducePow, beq_true]
+    rename_i v _
+    rw [←ith_def, ←isth_def] at v
+    assumption
+
+  · steps [CheckShuffle.check_shuffle_spec t_eq t_eq_spec]
+    rename_i ord perm _
+    rw [BitVec.toNat_sub_of_le (by assumption)] at ord
+    simp only [←n_eq_len, BitVec.toNat_intCast, Int.reducePow, Int.reduceMod, Int.toNat_one] at ord
+    rw [Nat.sub_add_cancel (by omega)] at ord
+    rw [List.take_length] at ord
+    exact ⟨ord, perm⟩
+
+  steps
+  subst_vars
+  assumption
+
+/--
+If it can be proven that the embedding of the comparator function is transitive, this theorem
+provides a stronger bound in that it states that the output is _strictly sorted_, and not only
+ordered by the provided relation.
+
+See `sort_via_spec` for a similar theorem that does not impose this restriction.
+-/
+theorem sort_via_trans_spec {p T N Env l f fb}
+    {t_eq : Cmp.Eq.hasImpl env T}
+    (t_eq_spec : ∀a b, STHoare p env ⟦⟧ (Cmp.Eq.eq h![] T h![] h![] h![a, b])
+      (fun r : Bool => ⟦r ↔ a = b⟧))
+    {fEmb : T.denote p → T.denote p → Bool}
+    (fEmb_trans : Transitive (fEmb · · = true))
+    (f_spec : ∀a b, STHoare p env ⟦⟧ (fb h![a, b]) (fun r => r = fEmb a b))
+  : STHoare p env [λf ↦ fb]
+    («std-1.0.0-beta.12::array::sort_via».call h![T, N, Env] h![l, f])
+    (fun r => List.Sorted (fEmb · · = true) r.toList ∧ List.Perm l.toList r.toList) := by
+  steps [sort_via_spec (t_eq := t_eq) t_eq_spec f_spec]
+  constructor
+  rename_i a
+  rcases a with ⟨ord_by, perm⟩
+  exact List.OrderedBy.trans_eq_Sorted ord_by fEmb_trans
+  simp_all
+
+/--
+This theorem asserts that `std::array::sort` implements a valid sort (namely that the output is
+a sorted permutation of the input) but does not make any requirements on _how_ the sort is done.
+
+It makes no guarantees as to the computational complexity or stability of the sort, but does ensure
+that the result is sorted by the provided relation and that its elements represent a valid
+permutation of the input.
+
+Do note that the function as written can only assume that the elements are pairwise ordered by the
+provided comparator function. In other words, it does **not** guarantee that they are sorted unless
+the comparator function is transitive. For a more strict version of this theorem, see
+`sort_trans_spec`, which uses a proof of transitivity for the `Ord` implementation to assure that
+the output is sorted.
+
+This theorem is pure, as we argue that there is no sensible use-case for impure `Ord` and `Eq`
+implementations for `T`.
+-/
+theorem sort_spec {p T N l}
+    {t_eq : Cmp.Eq.hasImpl env T}
+    (t_eq_spec : ∀a b, STHoare p env ⟦⟧ (Cmp.Eq.eq h![] T h![] h![] h![a, b])
+      (fun r : Bool => ⟦r ↔ a = b⟧))
+    {t_ord : Cmp.Ord.hasImpl env T}
+    (t_ord_emb : Tp.comparator p T)
+    (t_ord_spec : ∀a b, STHoare p env ⟦⟧ (Cmp.Ord.cmp h![] T h![] h![] h![a, b])
+      (fun r => r = Cmp.Ord.fromOrdering (t_ord_emb a b)))
+  : STHoare p env ⟦⟧
+    («std-1.0.0-beta.12::array::sort».call h![T, N] h![l])
+    (fun r => List.OrderedBy (Cmp.Ord.le_emb t_ord_emb · ·) r.toList
+      ∧ List.Perm l.toList r.toList) := by
+  enter_decl
+  steps
+
+  apply STHoare.consequence_frame
+  with_unfolding_all apply sort_via_spec
+  case h_ent => sl
+  case q_ent => intros; sl; assumption
+  any_goals assumption
+
+  intro a b
+  steps [t_ord_spec, Cmp.Ord.less_spec, Cmp.Ord.equal_spec, Cmp.Eq.ordering_eq_spec]
+  any_goals exact ()
+
+  subst_vars
+  rw [Cmp.Ord.fromOrdering_inj.eq_iff] at *
+  with_unfolding_all generalize toe_def : t_ord_emb a b = toe at *
+  congr <;> cases toe <;> simp_all
+
+/--
+If it can be proven that the embedding of the `Ord` implementation is transitive, this theorem
+provides a stronger bound in that it states that the output is _strictly sorted_, and not only
+ordered by the provided relation.
+
+See `sort_spec` for a similar theorem that does not impose this restriction.
+-/
+theorem sort_trans_spec {p T N l}
+    {t_eq : Cmp.Eq.hasImpl env T}
+    (t_eq_spec : ∀a b, STHoare p env ⟦⟧ (Cmp.Eq.eq h![] T h![] h![] h![a, b])
+      (fun r : Bool => ⟦r ↔ a = b⟧))
+    {t_ord : Cmp.Ord.hasImpl env T}
+    (t_ord_emb : Tp.comparator p T)
+    (t_ord_trans : Std.TransCmp t_ord_emb)
+    (t_ord_spec : ∀a b, STHoare p env ⟦⟧ (Cmp.Ord.cmp h![] T h![] h![] h![a, b])
+      (fun r => r = Cmp.Ord.fromOrdering (t_ord_emb a b)))
+  : STHoare p env ⟦⟧
+    («std-1.0.0-beta.12::array::sort».call h![T, N] h![l])
+    (fun r => List.Sorted (Cmp.Ord.le_emb t_ord_emb · ·) r.toList
+      ∧ List.Perm l.toList r.toList) := by
+  steps [sort_spec (t_eq := t_eq) t_eq_spec (t_ord := t_ord) t_ord_emb t_ord_spec]
+  constructor
+  rename_i a
+  rcases a with ⟨ord_by, perm⟩
+  apply List.OrderedBy.trans_eq_Sorted ord_by (Cmp.Ord.le_emb_trans t_ord_emb t_ord_trans)
+  simp_all
+
+theorem convert_from_str_spec {p N s}
+  : STHoare p env ⟦⟧
+    (Convert.«from» h![.str N] (.str N) h![] h![] h![s])
+    (fun r => r = s.bytes) := by
+  resolve_trait
+  steps
   simp_all
